coq/clc/clc_typing.v
@@ -9,82 +9,73 @@ Unset Printing Implicit Defensive.
 
 (** * Typing Rules of CLC *)
 
-Notation 𝐏 := (Sort U None).
 Reserved Notation "[ Γ |- ]".
 Reserved Notation "[ Γ |- m :- A ]".
 
 Inductive has_type : context term -> term -> term -> Prop :=
-| p_axiom Γ : 
-  [ Γ ] ->
-  [ Γ |- 𝐏 :- U @ 0 ]
 | s_axiom Γ s l : 
-  [ Γ ] ->
+  pure Γ ->
   [ Γ |- s @ l :- U @ l.+1 ]
-| prop Γ A B l :
-  [ Γ ] ->
-  [ Γ |- A :- Sort U l ] ->
-  [ A +u Γ |- B :- 𝐏 ] ->
-  [ Γ |- Arrow A B U :- 𝐏 ]
 | u_arrow Γ A B s l :
-  [ Γ ] ->
+  pure Γ ->
   [ Γ |- A :- U @ l ] ->
   [ A +u Γ |- B :- s @ l ] ->
   [ Γ |- Arrow A B U :- U @ l ]
 | l_arrow Γ A B s l :
-  [ Γ ] ->
+  pure Γ ->
   [ Γ |- A :- L @ l ] ->
-  [ □ Γ |- B :- s @ l ] ->
+  [ +n Γ |- B :- s @ l ] ->
   [ Γ |- Arrow A B L :- U @ l ]
 | u_lolli Γ A B s l :
-  [ Γ ] ->
+  pure Γ ->
   [ Γ |- A :- U @ l ] ->
   [ A +u Γ |- B :- s @ l ] ->
   [ Γ |- Lolli A B U :- L @ l ]
 | l_lolli Γ A B s l :
-  [ Γ ] ->
+  pure Γ ->
   [ Γ |- A :- L @ l ] ->
-  [ □ Γ |- B :- s @ l ] ->
+  [ +n Γ |- B :- s @ l ] ->
   [ Γ |- Lolli A B L :- L @ l ]
 | u_var Γ x A : 
-  [ x :u A ∈ Γ ] ->
+  hasU Γ x A ->
   [ Γ |- Var x :- A ]
 | l_var Γ x A :
-  [ x :l A ∈ Γ ] ->
+  hasL Γ x A ->
   [ Γ |- Var x :- A ]
 | arrow_lam Γ n A B s t l :
-  [ Γ ] ->
-  [ Γ |- Arrow A B s :- Sort t l ] ->
+  pure Γ ->
+  [ Γ |- Arrow A B s :- t @ l ] ->
   [ A +{s} Γ |- n :- B ] ->
   [ Γ |- Lam A n s :- Arrow A B s ]
 | lolli_lam Γ n A B s t l :
-  [ %Γ |- Lolli A B s :- Sort t l ] ->
+  [ re Γ |- Lolli A B s :- t @ l ] ->
   [ A +{s} Γ |- n :- B ] ->
   [ Γ |- Lam A n s :- Lolli A B s ]
 | u_arrow_app Γ1 Γ2 Γ A B m n :
-  [ Γ2 ] ->
+  pure Γ2 ->
   [ Γ1 |- m :- Arrow A B U ] ->
   [ Γ2 |- n :- A ] ->
-  [ Γ1 ‡ Γ2 ‡ Γ ] ->
+  merge Γ1 Γ2 Γ ->
   [ Γ |- App m n :- B.[n/] ]
 | l_arrow_app Γ1 Γ2 Γ  A B m n :
   [ Γ1 |- m :- Arrow A B L ] ->
   [ Γ2 |- n :- A ] ->
-  [ Γ1 ‡ Γ2 ‡ Γ ] ->
+  merge Γ1 Γ2 Γ ->
   [ Γ |- App m n :- B.[n/] ]
 | u_lolli_app Γ1 Γ2 Γ A B m n :
-  [ Γ2 ] ->
+  pure Γ2 ->
   [ Γ1 |- m :- Lolli A B U ] ->
   [ Γ2 |- n :- A ] ->
-  [ Γ1 ‡ Γ2 ‡ Γ ] ->
+  merge Γ1 Γ2 Γ ->
   [ Γ |- App m n :- B.[n/] ]
 | l_lolli_app Γ1 Γ2 Γ  A B m n :
   [ Γ1 |- m :- Lolli A B L ] ->
   [ Γ2 |- n :- A ] ->
-  [ Γ1 ‡ Γ2 ‡ Γ ] ->
+  merge Γ1 Γ2 Γ ->
   [ Γ |- App m n :- B.[n/] ]
 | conversion Γ A B m s l :
   A <: B ->
-  [ %Γ |- B :- Sort s l ] ->
+  [ re Γ |- B :- Sort s l ] ->
   [ Γ |- m :- A ] ->
   [ Γ |- m :- B ]
 where "[ Γ |- m :- A ]" := (has_type Γ m A).
@@ -94,20 +85,20 @@ Inductive context_ok : context term -> Prop :=
   [ nil |- ]
 | u_ok Γ A l :
   [ Γ |- ] ->
-  [ %Γ |- A :- Sort U l ] ->
+  [ re Γ |- A :- Sort U l ] ->
   [ A +u Γ |- ]
 | l_ok Γ A l :
   [ Γ |- ] ->
-  [ %Γ |- A :- Sort L l ] ->
+  [ re Γ |- A :- Sort L l ] ->
   [ A +l Γ |- ]
 | n_ok Γ :
   [ Γ |- ] ->
-  [ □ Γ |- ]
+  [ +n Γ |- ]
 where "[ Γ |- ]" := (context_ok Γ).
 
 Lemma re_ok Γ :
   [ Γ |- ] ->
-  [ %Γ |- ].
+  [ re Γ |- ].
 Proof with eauto using context_ok.
   intros.
   induction H...
