coq/clc/clc_validity.v
@@ -13,7 +13,7 @@ Unset Printing Implicit Defensive.
   Types of well-typed terms are themselves well-sorted. *)
 
 Lemma merge_context_ok_inv Γ Γ1 Γ2 :
-  [ Γ1 ‡ Γ2 ‡ Γ ] ->
+  merge Γ1 Γ2 Γ ->
   [ Γ |- ] ->
   [ Γ1 |- ] /\ [ Γ2 |- ].
 Proof.
@@ -50,29 +50,23 @@ Qed.
 Theorem validity Γ m A : 
   [ Γ |- ] ->
   [ Γ |- m :- A ] ->
-  exists s l, [ %Γ |- A :- Sort s l ].
+  exists s l, [ re Γ |- A :- Sort s l ].
 Proof.
   intros.
   dependent induction H0.
-  - exists U; exists (Some 1).
+  - exists U; exists l.+2.
     constructor.
     rewrite <- pure_re; eauto.
-  - exists U; exists (Some l.+2).
+  - exists U; exists l.+1.
     constructor.
     rewrite <- pure_re; eauto.
-  - exists U; exists (Some 0).
+  - exists U; exists l.+1.
     constructor.
     rewrite <- pure_re; eauto.
-  - exists U; exists (Some l.+1).
+  - exists U; exists l.+1.
     constructor.
     rewrite <- pure_re; eauto.
-  - exists U; exists (Some l.+1).
-    constructor.
-    rewrite <- pure_re; eauto.
-  - exists U; exists (Some l.+1).
-    constructor.
-    rewrite <- pure_re; eauto.
-  - exists U; exists (Some l.+1).
+  - exists U; exists l.+1.
     constructor.
     rewrite <- pure_re; eauto.
   - exists U.
@@ -89,7 +83,7 @@ Proof.
     exists x3; exists x4.
     replace (Sort x3 x4) with ((Sort x3 x4).[n/]) by autosubst.
     eapply substitutionU; eauto.
-    replace (Γ2) with (%Γ1).
+    replace (Γ2) with (re Γ1).
     apply merge_re_re_re.
     apply pure_re in H0.
     rewrite H0.
@@ -121,21 +115,4 @@ Proof.
     eapply substitutionN; eauto.
     rewrite <- H2; eauto.
   - exists s; exists l; eauto.
-Qed.
-
-Lemma propL_false Γ A :
-  ~[ Γ |- Sort L None :- A ].
-Proof.
-  intro H.
-  dependent induction H.
-  apply IHhas_type2; eauto.
-Qed.
-
-Lemma has_propL_false Γ m :
-  [ Γ |- ] -> [ Γ |- m :- Sort L None ] -> False.
-Proof.
-  intros.
-  apply validity in H0; eauto. 
-  first_order.
-  apply propL_false in H0; eauto.
 Qed.
